minuska-examples/theories/examples_unary_nat.v
@@ -185,16 +185,16 @@ Module unary_nat.
     Fixpoint unary_to_nat'
         (g : PreTerm' symbol builtin_value) : option nat :=
     match g with
-    | ao_operator "nat_zero" => Some 0
-    | ao_app_ao (ao_operator "nat_succ") g' => n ← (unary_to_nat' g'); Some (S n)
+    | pt_operator "nat_zero" => Some 0
+    | pt_app_ao (pt_operator "nat_succ") g' => n ← (unary_to_nat' g'); Some (S n)
     | _ => None
     end
     .
 
     Definition unary_to_nat (g : GroundTerm) : option nat :=
     match g with
-    | aoo_app ao => unary_to_nat' ao
-    | aoo_operand _ => None
+    | term_preterm ao => unary_to_nat' ao
+    | term_operand _ => None
     end
     .
 
@@ -204,12 +204,12 @@ Module unary_nat.
 
     Definition final (g : GroundTerm) : option nat :=
     match g with
-    |  aoo_app 
-        (ao_app_ao 
-            (ao_operator "u_cfg")
-            (ao_app_ao 
-                (ao_app_ao 
-                    (ao_operator "u_cseq")
+    |  term_preterm 
+        (pt_app_ao 
+            (pt_operator "u_cfg")
+            (pt_app_ao 
+                (pt_app_ao 
+                    (pt_operator "u_cseq")
                     val
                 )
                 _
